SP1CleanTest/Core/HostChecks.lean
@@ -82,7 +82,7 @@ def evaluateProgram (program : Circuit Fp Unit) (inputs : List Fp)
             0 < a.val + b.val * 65536 + c.val * 65536 ^ 2 && (last == 0 || last == 1)
         | _ => false
       else ["sp1.native.hint_queue_state", "sp1.native.hint_read_state", "SP1WritePermission",
-        "SP1State", "SP1Exit", "SP1Syscall", "SP1PublicValues", "sp1.native.host_call",
+        "SP1State", "SP1Exit", "SP1HostExit", "SP1Syscall", "SP1PublicValues", "sp1.native.host_call",
         "sp1.native.commit_state", "sp1.native.deferred_state", "sp1.native.host_ram_access"].contains
           interaction.channel.name
   (valid, (FlatOperation.interactions operations).filterMap fun interaction =>
